feat: automatic linkifier (#183)
This is JS that transforms entries in the Verso xref table into actual
links or redirects. This will be suitable for incoming links from
docstrings or Zulip.

static-web/find.js
@@ -1,0 +1,61 @@
+let params = new URLSearchParams(document.location.search);
+let domains = params.getAll("domain");
+let target = params.get("target");
+console.log("Domains: " + domains);
+console.log("target: " + target);
+if(target) {
+    let options = [];
+    if (domains && domains.length > 0) {
+        for (const i in domains) {
+            let domain = domains[i];
+            console.log('Considering domain ' + domain);
+            if (xref.hasOwnProperty(domain)) {
+                console.log('Found domain ' + domain);
+                let opts = xref[domain];
+                if (opts['contents'].hasOwnProperty(target)) {
+                    options = opts['contents'][target].map(x => Object.assign(x, {'domain': domain}));
+                }
+            }
+        }
+    } else {
+        for (const [dom, opts] of Object.entries(xref)) {
+            if (opts['contents'].hasOwnProperty(target)) {
+                for (const i of opts['contents'][target]) {
+                    options.push(Object.assign(i, {'domain': dom}));
+                }
+            }
+        }
+    }
+
+    if (options.length == 0) {
+        addEventListener('DOMContentLoaded', event => {
+            document.title = "Not found: '" + target + "'";
+            document.querySelector("#title").innerHTML = "Not found: target '" + target + "'";
+            let allDomains = [];
+            for (const d in xref) {
+                allDomains.push(d);
+            }
+            if (domains.length < 1) {
+                domains = allDomains;
+            }
+            document.querySelector("#message").innerHTML = "<p>Searched domains:</p>" + "<ul>" + domains.map(x => "<li><code>" + x + "</code>: " + xref[x]['title'] + "</li>\n").join('') + "</ul>";
+        });
+    } else if (options.length == 1) {
+        let addr = options[0]['address'] + "#" + options[0]['id'];
+        window.location.replace(addr);
+    } else {
+        addEventListener('DOMContentLoaded', event => {
+            document.title = "Ambiguous: '" + target + "'";
+            document.querySelector("#title").innerHTML = "Ambiguous: target '" + target + "'";
+            document.querySelector("#message").innerHTML = "<p>Options:</p><ul>" +
+                options.map((x, idx) => '<li><p><a href="' + x['address'] + '#' + x['id'] + '">From ' + xref[x['domain']]['title'] + '</a></p></li>').join('\n') +
+                "</ul>";
+        });
+    }
+} else {
+    addEventListener('DOMContentLoaded', event => {
+        document.title = "No target provided";
+        document.querySelector("#title").innerHTML = "No target provided";
+        document.querySelector("#message").innerHTML = "<p>This script expects a 'target' query parameter, along with documentation domains.</p>";
+    });
+}
