src/verso-manual/VersoManual/WebAssets.lean
@@ -1,0 +1,8 @@
+/-
+Copyright (c) 2024 Lean FRO LLC. All rights reserved.
+Released under Apache 2.0 license as described in the file LICENSE.
+Author: David Thrane Christiansen
+-/
+namespace Verso.Genre.Manual
+
+def find.js := include_str "../../../static-web/find.js"
